\documentclass[preview]{standalone}
\usepackage[english]{babel}
\usepackage{amsmath}
\usepackage{amssymb}
\begin{document}
\begin{align*}
T_{3}&= \int_{0}^{+1}t e^{-i\omega t} \ dt \\&=\left[\frac{e^{-i\omega t}(1+i\omega t)}{\omega^{2}}\right]_{0}^{+1} \\ &=\frac{e^{-i\omega\cdot 1}(1+i\omega\cdot 1)}{\omega^{2}}-\frac{e^{-i\omega\cdot 0}(1+i\omega\cdot 0)}{\omega^{2}} \\ &=\frac{e^{-i\omega}(1+i\omega)-1(1+0)}{\omega^{2}} \\ &= &=\frac{e^{-i\omega}(1+i\omega)-1}{\omega^{2}}
\end{align*}
\end{document}