\documentclass[preview]{standalone}
\usepackage[english]{babel}
\usepackage{amsmath}
\usepackage{amssymb}
\begin{document}
\begin{align*}
F(\omega)&=T_{1}+T_{2}-T_{3} \\ &=\frac{i(e^{-i\omega}-e^{i\omega})}{\omega}+\frac{1-e^{i\omega}(1-i\omega)}{\omega^{2}}-\frac{e^{-i\omega}(1+i\omega)-1}{\omega^{2}} \\ &=\frac{i\omega(e^{-i\omega}-e^{i\omega})+1-e^{i\omega}(1-i\omega)-e^{-i\omega}(1+i\omega)+1}{\omega^{2}} \\ &=\frac{i\omega e^{-i\omega}-i\omega e^{i\omega}+1-e^{i\omega}+i\omega e^{i\omega}-e^{-i\omega}-i\omega e^{-i\omega}+1}{\omega^{2}} \\ &=\frac{2-e^{i\omega} - e^{-i\omega}}{\omega^{2}} \\ &=\frac{2-(e^{i\omega}+e^{-i\omega})}{\omega^{2}} \quad \textrm{Using} \quad 2\cos{\theta} =e^{i\theta}+e^{-i\theta}; \\ &=\frac{2-2\cos{(\omega)}}{\omega^{2}} = 2\big[\frac{1-\cos{(\omega)}}{\omega^{2}}\big] \\ &=\textrm{Using} \quad 1-\cos{\theta}=2\sin^{2}{\big( \frac{\theta}{2} \big) }; \\ &=4\big{ \frac{\sin^{2}{\big[ \pi \big( \frac{\omega}{2\pi} \big) \big]}}{4\big{\big[ \pi \big( \frac{\omega}{2\pi} \big) \big]^{2} \big} \\ \textrm{sinc}^{2}\big( \frac{\omega}{2\pi} \big)}}
\end{align*}
\end{document}