\documentclass[preview]{standalone}
\usepackage[english]{babel}
\usepackage{amsmath}
\usepackage{amssymb}
\begin{document}
\begin{align*}
T_{2}&= \int_{-1}^{0}t e^{-i\omega t} \ dt \\ &=\left[\frac{e^{-i\omega t}(1+i\omega t)}{\omega^{2}}\right]_{-1}^{0} \\ &=\frac{e^{-i\omega\cdot 0}(1+i\omega\cdot 0)}{\omega^{2}}-\frac{e^{-i\omega\cdot -1}(1+i\omega\cdot -1)}{\omega^{2}} \\ &=\frac{1(1+0)-e^{i\omega}(1-i\omega)}{\omega^{2}} \\ &= \frac{1-e^{i\omega}(1-i\omega)}{\omega^{2}}
\end{align*}
\end{document}